Made progress on compilation with Ruxandra

state/SimpleState.fst
@@ -5,9 +5,10 @@ open FStar.Ref
 assume val trp : Type // Type of the reference of the program (not shared)
 assume val trs : Type // Type of the reference *shared* between program and context
                       // <- for now let's assume this is not refined
-assume val t1 : Type  // Type not allowed to contain references,
+                      // (assumed for all the types here, since they are used in target)
+assume val targ : Type// Type not allowed to contain references,
                       // since otherwise the program can share `rp` to the context.
-assume val t2 : Type
+assume val tres : Type
 
 // Simple target types
 
@@ -15,24 +16,28 @@ assume val t2 : Type
 let t_tw : Type = ref trp -> ref trs -> St int
 
 // Target type of context
-let t_tc : Type = ref trs -> t1 -> St t2
+let t_tc : Type = ref trs -> targ -> St tres
 
 // Target type of program -- has initial control, calls context
-let t_tp : Type = ref trp -> ref trs -> (t1 -> St t2) -> St int
+let t_tp : Type = ref trp -> ref trs -> (targ -> St tres) -> St int
 
 let t_link (t_p:t_tp) (t_c:t_tc) : t_tw =
   fun (rp:ref trp) (rs:ref trs) ->
-    t_p rp rs (t_c rs)
+    t_p rp rs (t_c rs) (* <-- rp is not passed to the context *)
 
-// Refined source types
+// Refined source types (pre- and post-conditions on stateful functions)
 
 // This separation invariant used for both program and context
-let sep (rp:ref trp) (rs:ref trs) (h0:heap) : Type0 =
+let sep (rp:ref trp) (rs:ref trs) (h:heap) : Type0 =
   (* initial references are not aliasing: (what hyper-heap regions could give us?) *)
   addr_of rp <> addr_of rs /\
   (* initial references are allocated: *)
-  h0 `contains` rp /\ h0 `contains` rs
+  h `contains` rp /\ h `contains` rs
   (* + TODO (hard in general!?): rp is not reachable from rs *)
+  (* Does this kind of (un)reachability (deep/transitive) already lead us to
+     separation logic, or is there anything we can do in a simpler setting. *)
+  (* Otherwise can define unreachability predicate for specific types like
+     linked lists *)
 
 assume val post_prog : ref trp -> ref trs -> heap -> int -> heap -> Type0
 // <- user defined and proved statically about the partial program
@@ -41,25 +46,30 @@ let s_tw : Type = rp:ref trp -> rs:ref trs ->
   ST int (requires (fun h0 -> sep rp rs h0))
          (ensures (fun h0 res h1 -> post_prog rp rs h0 res h1))
 
-assume val pre_ctx : ref trs -> t1 -> heap -> Type0
+assume val pre_ctx : ref trs -> targ -> heap -> Type0
 // <- user defined and proved statically about the partial program (who calls context)
 
-assume val post_ctx : ref trs -> t1 -> heap -> t2 -> heap -> bool
+assume val post_ctx : ref trs -> targ -> heap -> tres -> heap -> bool
 // dynamically enforced when the context returns control back to the program
 // (so for now going directly to bool)
+// TODO: Cezar worried that enforcing this is difficult.
+//       In FStar.ST.fst we do have a way to get the heap (gst_get),
+//       but this will cause extraction problems later on
+// - Saner longer term alternative :
+//   look only at value of rs in initial and final heap?
 
-let s_tc (rp:ref trp) : Type = rs:ref trs -> arg:t1 ->
-  ST t2 (requires (fun h0 -> sep rp rs h0 /\ pre_ctx rs arg h0))
-        (ensures (fun h0 res h1 -> sep rp rs h1 // <- necessarily preserved by context
-          /\ post_ctx rs arg h0 res h1 // <- dynamically enforced
-          /\ sel h0 rp == sel h1 rp)) // <- enforced by state separation
+let s_tc (rp:ref trp) : Type = rs:ref trs -> arg:targ ->
+  ST tres (requires (fun h0 -> sep rp rs h0 /\ pre_ctx rs arg h0))
+          (ensures (fun h0 res h1 -> sep rp rs h1 // <- necessarily preserved by context
+            /\ post_ctx rs arg h0 res h1 // <- dynamically enforced
+            /\ sel h0 rp == sel h1 rp)) // <- enforced by state separation
 
 // putting together the types + specs above
 let s_tp : Type = rp:ref trp -> rs:ref trs ->
-  (arg:t1 -> ST t2 (requires (fun h0 -> sep rp rs h0 /\ pre_ctx rs arg h0))
-                   (ensures (fun h0 res h1 -> sep rp rs h1
-                     /\ post_ctx rs arg h0 res h1
-                     /\ sel h0 rp == sel h1 rp))) ->
+  (arg:targ -> ST tres (requires (fun h0 -> sep rp rs h0 /\ pre_ctx rs arg h0))
+                       (ensures (fun h0 res h1 -> sep rp rs h1
+                       /\ post_ctx rs arg h0 res h1
+                       /\ sel h0 rp == sel h1 rp))) ->
   ST int (requires (fun h0 -> sep rp rs h0))
          (ensures (fun h0 res h1 -> post_prog rp rs h0 res h1))
 
@@ -74,12 +84,31 @@ let s_link (s_p:s_tp) (rp:ref trp) (s_c:s_tc rp) (rs:ref trs) :
 
 open FStar.Ghost
 
-let se_tc : Type = erp:erased (ref trp) -> rs:ref trs -> arg:t1 ->
-  ST t2 (requires (fun h0 -> sep erp rs h0 /\ pre_ctx rs arg h0))
-        (ensures (fun h0 res h1 -> sep erp rs h1 // <- necessarily preserved by context
-          /\ post_ctx rs arg h0 res h1 // <- dynamically enforced
-          /\ sel h0 erp == sel h1 erp)) // <- enforced by state separation
+let se_tc : Type = erp:erased (ref trp) -> rs:ref trs -> arg:targ ->
+  ST tres (requires (fun h0 -> sep erp rs h0 /\ pre_ctx rs arg h0))
+          (ensures (fun h0 res h1 -> sep erp rs h1 // <- necessarily preserved by context
+            /\ post_ctx rs arg h0 res h1 // <- dynamically enforced
+            /\ sel h0 erp == sel h1 erp)) // <- enforced by state separation
 
 let se_link (s_p:s_tp) (s_c:se_tc) : s_tw =
   fun (rp:ref trp) (rs:ref trs) ->
-    s_p rp rs (s_c rp rs)
+    s_p rp rs (s_c rp rs) (* rp passed to the context, but only as `erased` argument *)
+
+let compile (s_p:s_tp) : t_tp =
+  fun rp rs t_c -> 
+    let s_c arg : ST tres (requires (fun h0 -> sep rp rs h0 /\ pre_ctx rs arg h0))
+                          (ensures (fun h0 res h1 -> sep rp rs h1
+                          /\ post_ctx rs arg h0 res h1
+                          /\ sel h0 rp == sel h1 rp)) =
+      let h0 = gst_get() in
+      let res = t_c arg in
+      let h1 = gst_get() in
+      assume (sep rp rs h1); // TODO: seems hard
+      assume (sel h0 rp == sel h1 rp); // TODO: seems hard
+      if post_ctx rs arg h0 res h1
+      then res
+      else admit() // TODO: signal error :)
+    in
+    let h0 = gst_get() in
+    assume (sep rp rs h0); // TODO: where would one get initial separation from?
+    s_p rp rs s_c
