state/LinkedList.fst
@@ -1,0 +1,15 @@
+module LinkedList
+
+(* With `open FStar.Ref` and just using ref below we get *)
+(* Inductive type `list` does not satisfy the strict positivity condition *)
+
+(* However, the `mref` type in `FStar.Monotonic.Heap` is defined to
+   be strictly positive, which makes the following code work: *)
+
+open FStar.Monotonic.Heap
+open FStar.Heap
+
+noeq type linked (a:Type0) : Type0 =
+  | Nil
+  | Cons of a * ref (linked a)
+
